pancake-structs: unsafe mode, proof repairs
Add a switch that controls the "safety" of the pancake named-structs features.
The idea is to get to the point where the main proofs are repaired, and the
named-structs features are installed but aren't considered safe for verified
code.

Repair panSem and panProps proofs for the additional types and ops. The fact
that the safety switch is set to off hasn't actually been used yet.

pancake/semantics/panPropsScript.sml
@@ -12,33 +12,63 @@ Definition v2word_def:
   v2word (ValWord v) = Word v
 End
 
+Definition no_named_shape_def:
+  no_named_shape (Named nm) = F /\
+  no_named_shape One = T /\
+  no_named_shape (Comb xs) = EVERY no_named_shape xs
+End
+
+Theorem shape_of_val:
+  shape_of (Val x) = One
+Proof
+  Cases_on `x` \\ simp [shape_of_def]
+QED
+
 Theorem length_flatten_eq_size_of_shape:
-  !v.
+  !v. no_named_shape (shape_of v) ==>
    LENGTH (flatten v) = size_of_shape (shape_of v)
 Proof
-  ho_match_mp_tac flatten_ind >> rw []
-  >- (cases_on ‘w’ >> fs [shape_of_def, flatten_def, size_of_shape_def]) >>
-  fs [shape_of_def, flatten_def, size_of_shape_def] >>
-  fs [LENGTH_FLAT, MAP_MAP_o] >> fs[SUM_MAP_FOLDL] >>
-  match_mp_tac FOLDL_CONG >> fs []
+  recInduct flatten_ind >> rw [] >>
+  fs [no_named_shape_def, shape_of_def, shape_of_val] >>
+  simp [flatten_def, shape_of_def, size_of_shape_def] >>
+  simp [LENGTH_FLAT, MAP_MAP_o, o_DEF] >>
+  fs[SUM_MAP_FOLDL] >>
+  match_mp_tac FOLDL_CONG >> fs [] >>
+  fs [EVERY_MAP] >> fs [EVERY_MEM]
+QED
+
+Theorem dropWhile_eq_cons_IMP[local]:
+  dropWhile P xs = y :: ys ==> ~ P y
+Proof
+  Induct_on `xs` \\ rw [dropWhile_def]
+  \\ simp []
+QED
+
+Theorem mem_loads_some_shape_eq:
+  (∀sh adr dm (m: 'a word -> 'a word_lab) stcs v.
+  mem_load sh adr dm m stcs = SOME v ==> shape_of v = sh) /\
+  (∀shs adr dm (m: 'a word -> 'a word_lab) stcs vs.
+   mem_loads shs adr dm m stcs = SOME vs ==> MAP shape_of vs = shs) /\
+  (∀flds adr dm (m: 'a word -> 'a word_lab) stcs vs.
+   mem_load_flds flds adr dm m stcs = SOME vs ==>
+    MAP (shape_of o SND) vs = MAP SND flds)
+Proof
+  ho_match_mp_tac mem_load_ind
+  \\ rw [mem_load_def]
+  \\ fs [shape_case_eq, option_case_eq, list_case_eq, pair_case_eq]
+  \\ imp_res_tac dropWhile_eq_cons_IMP \\ fs []
+  \\ rw [shape_of_def, shape_of_val]
+  \\ fs []
+  \\ simp_tac (bool_ss ++ ETA_ss) []
 QED
 
 Theorem mem_load_some_shape_eq:
-  ∀sh adr dm (m: 'a word -> 'a word_lab) v.
-  mem_load sh adr dm m = SOME v ==>
+  ∀sh adr dm (m: 'a word -> 'a word_lab) stcs v.
+  mem_load sh adr dm m stcs = SOME v ==>
   shape_of v = sh
 Proof
-  qsuff_tac ‘(∀sh adr dm (m: 'a word -> 'a word_lab) v.
-  mem_load sh adr dm m = SOME v ==> shape_of v = sh) /\
-  (∀sh adr dm (m: 'a word -> 'a word_lab) v.
-   mem_loads sh adr dm m = SOME v ==> MAP shape_of v = sh)’
-  >- metis_tac [] >>
-  ho_match_mp_tac mem_load_ind >> rw [mem_load_def] >>
-  cases_on ‘sh’ >> fs [option_case_eq] >>
-  rveq >> TRY (cases_on ‘m adr’) >> fs [shape_of_def] >>
-  metis_tac []
+  metis_tac [mem_loads_some_shape_eq]
 QED
-
 
 Theorem flookup_res_var_some_eq_lookup:
   FLOOKUP (res_var lc (v,FLOOKUP lc' v)) v = SOME value ==>
@@ -64,10 +94,11 @@ Proof
   rw[DOMSUB_FLOOKUP_THM,FLOOKUP_UPDATE]
 QED
 
-Theorem list_rel_length_shape_of_flatten:
+Theorem list_rel_length_shape_of_flatten_better[local]:
   !vshs args.
-  LIST_REL (λvsh arg. SND vsh = shape_of arg) vshs args ==>
-  size_of_shape (Comb (MAP SND vshs)) = LENGTH (FLAT (MAP flatten args))
+  LIST_REL (λvsh arg. vsh = shape_of arg) vshs args /\
+  EVERY (no_named_shape) vshs ==>
+  size_of_shape (Comb vshs) = LENGTH (FLAT (MAP flatten args))
 Proof
   Induct >> rpt gen_tac >> strip_tac
   >- (cases_on ‘args’ >> fs [size_of_shape_def]) >>
@@ -79,6 +110,14 @@ Proof
   fs [length_flatten_eq_size_of_shape]
 QED
 
+Theorem list_rel_length_shape_of_flatten:
+  !vshs args.
+  LIST_REL (λvsh arg. SND vsh = shape_of arg) vshs args /\
+  EVERY (no_named_shape o SND) vshs ==>
+  size_of_shape (Comb (MAP SND vshs)) = LENGTH (FLAT (MAP flatten args))
+Proof
+  simp [list_rel_length_shape_of_flatten_better, EVERY_MAP, o_DEF, LIST_REL_MAP]
+QED
 
 Theorem length_with_shape_eq_shape:
   !sh ns.
@@ -369,7 +408,8 @@ Theorem list_rel_flatten_with_shape_length:
   LENGTH ns = LENGTH (FLAT (MAP flatten args))/\
   size_of_shape (Comb sh) = LENGTH (FLAT (MAP flatten args)) /\
   EL n args = v /\ n < LENGTH args /\ LENGTH args = LENGTH sh /\
-  LIST_REL (λsh arg. sh = shape_of arg) sh args ==>
+  LIST_REL (λsh arg. sh = shape_of arg) sh args /\
+  EVERY no_named_shape sh ==>
   LENGTH (EL n (with_shape sh ns)) = LENGTH (flatten v)
 Proof
   Induct >> rw []
@@ -383,114 +423,63 @@ Proof
   fs []
 QED
 
+Theorem el_el_with_shape:
+  LENGTH xs = size_of_shape (Comb shs) /\
+  n < LENGTH shs /\ n' < size_of_shape (EL n shs) /\
+  EVERY no_named_shape shs ==>
+  EL n' (EL n (with_shape shs xs)) =
+  EL (n' + size_of_shape (Comb (TAKE n shs))) xs
+Proof
+  simp [with_shape_el_take_drop_eq]
+  \\ rw [EL_TAKE]
+  \\ irule EL_DROP
+  \\ simp []
+  \\ qspecl_then [`shs`, `n`] assume_tac LESS_LENGTH
+  \\ gs [TAKE_APPEND1, TAKE_APPEND2, TAKE_LENGTH_TOO_LONG]
+  \\ fs [EL_APPEND1, EL_APPEND2]
+  \\ simp [size_of_shape_def, SUM_APPEND]
+QED
+
 Theorem list_rel_flatten_with_shape_flookup:
   !sh ns args v n n'.
   ALL_DISTINCT ns ∧ LENGTH ns = LENGTH (FLAT (MAP flatten args)) /\
   size_of_shape (Comb sh) = LENGTH (FLAT (MAP flatten args)) /\
   EL n args = v /\ n < LENGTH args /\ LENGTH args = LENGTH sh /\
   LIST_REL (λsh arg. sh = shape_of arg) sh args /\
+  EVERY no_named_shape sh /\
   LENGTH (EL n (with_shape sh ns)) = LENGTH (flatten v) /\
   n' < LENGTH (EL n (with_shape sh ns)) ==>
    FLOOKUP (FEMPTY |++ ZIP (ns,FLAT (MAP flatten args)))
      (EL n' (EL n (with_shape sh ns))) =
    SOME (EL n' (flatten v))
 Proof
-  Induct >> rw []
-  >- fs [with_shape_def, size_of_shape_def] >>
-  fs [with_shape_def, size_of_shape_def] >>
-  cases_on ‘n’ >> fs []
-  >- (
-   ‘FLOOKUP (FEMPTY |++ ZIP (ns,flatten arg ++ FLAT (MAP flatten ys)))
-    (EL n' (TAKE (size_of_shape (shape_of arg)) ns)) =
-    SOME (EL n' (flatten arg ++ FLAT (MAP flatten ys)))’ by (
-     ‘size_of_shape (shape_of arg) = LENGTH (flatten arg)’ by
-       fs [length_flatten_eq_size_of_shape] >>
-     fs [] >>
-     ‘EL n' (flatten arg ++ FLAT (MAP flatten ys)) = EL n' (flatten arg)’ by (
-       match_mp_tac EL_APPEND1 >> fs []) >>
-     fs [] >>
-     ‘FEMPTY |++ ZIP (TAKE (LENGTH (flatten arg)) ns ++ DROP (LENGTH (flatten arg)) ns,
-                      flatten arg ++ FLAT (MAP flatten ys)) =
-      FEMPTY |++ ZIP (TAKE (LENGTH (flatten arg)) ns,flatten arg) |++
-      ZIP (DROP (LENGTH (flatten arg)) ns,FLAT (MAP flatten ys))’ by (
-       drule ZIP_APPEND >>
-       disch_then (qspecl_then [‘DROP (LENGTH (flatten arg)) ns’, ‘FLAT (MAP flatten ys)’]mp_tac) >>
-       impl_tac >- fs [] >>
-       strip_tac >> pop_assum (assume_tac o GSYM) >>
-       fs [] >>
-       fs [FUPDATE_LIST_APPEND]) >>
-     fs [] >> pop_assum kall_tac >>
-     ‘FEMPTY |++ ZIP (TAKE (LENGTH (flatten arg)) ns,flatten arg) |++
-      ZIP (DROP (LENGTH (flatten arg)) ns,FLAT (MAP flatten ys)) =
-      FEMPTY  |++
-      ZIP (DROP (LENGTH (flatten arg)) ns,FLAT (MAP flatten ys)) |++
-      ZIP (TAKE (LENGTH (flatten arg)) ns,flatten arg)’ by (
-       match_mp_tac FUPDATE_LIST_APPEND_COMMUTES >>
-       fs [MAP_ZIP] >> match_mp_tac all_distinct_take_frop_disjoint >> fs []) >>
-     fs [] >> pop_assum kall_tac >>
-     match_mp_tac update_eq_zip_flookup >>
-     fs [] >>
-     match_mp_tac all_distinct_take >>
-     fs []) >>
-   fs [] >>
-   pop_assum kall_tac >>
-   metis_tac [EL_APPEND1]) >>
-  ‘FLOOKUP (FEMPTY |++ ZIP (ns,flatten arg ++ FLAT (MAP flatten ys)))
-    (EL n'
-     (EL n'' (with_shape sh (DROP (size_of_shape (shape_of arg)) ns))))  =
-    FLOOKUP (FEMPTY |++ ZIP (DROP (size_of_shape (shape_of arg)) ns,FLAT (MAP flatten ys)))
-    (EL n'
-     (EL n'' (with_shape sh (DROP (size_of_shape (shape_of arg)) ns))))’ by (
-    ‘FEMPTY |++ ZIP (ns,flatten arg ++ FLAT (MAP flatten ys)) =
-     FEMPTY  |++
-     ZIP (TAKE (LENGTH (flatten arg)) ns,flatten arg) |++
-     ZIP (DROP (LENGTH (flatten arg)) ns,FLAT (MAP flatten ys))’ by (
-      match_mp_tac fm_zip_append_take_drop >>
-      fs []) >>
-    fs [] >> pop_assum kall_tac >>
-    ‘FLOOKUP
-     (FEMPTY |++ ZIP (TAKE (LENGTH (flatten arg)) ns,flatten arg))
-     (EL n'
-      (EL n'' (with_shape sh (DROP (size_of_shape (shape_of arg)) ns)))) = NONE’ by (
-      match_mp_tac not_mem_fst_zip_flookup_empty >>
-      fs [] >> drule all_distinct_take >> disch_then (qspec_then ‘LENGTH (flatten arg)’ assume_tac) >>
-      fs [] >>
-      CCONTR_TAC >> fs [] >>
-      fs [GSYM length_flatten_eq_size_of_shape] >>
-      ‘TAKE (LENGTH (flatten arg)) ns =
-       EL 0 (with_shape (shape_of arg::sh) ns)’ by
-        fs [with_shape_def, length_flatten_eq_size_of_shape] >>
-      ‘EL n'' (with_shape sh (DROP (LENGTH (flatten arg)) ns)) =
-       EL (SUC n'') (with_shape (shape_of arg::sh) ns)’ by
-        fs [with_shape_def, length_flatten_eq_size_of_shape] >>
-      drule all_distinct_disjoint_with_shape >>
-      disch_then (qspecl_then [‘shape_of arg::sh’, ‘SUC n''’, ‘0’] mp_tac) >>
-      impl_tac >- fs [length_flatten_eq_size_of_shape, size_of_shape_def] >>
-      strip_tac >> fs [] >> drule disjoint_not_mem_el >> metis_tac []) >>
-    drule fupdate_flookup_zip_elim >>
-    disch_then (qspecl_then [‘DROP (LENGTH (flatten arg)) ns’, ‘FLAT (MAP flatten ys)’] mp_tac) >>
-    impl_tac >- (fs [] >> match_mp_tac all_distinct_take >> fs []) >>
-    fs [] >> strip_tac >>
-    fs [length_flatten_eq_size_of_shape]) >>
-  fs [] >>
-  pop_assum kall_tac >>
-  last_x_assum (qspecl_then [‘DROP (size_of_shape (shape_of arg)) ns’,
-                             ‘ys’, ‘n''’, ‘n'’] mp_tac) >>
-  impl_tac >-  fs [ALL_DISTINCT_DROP, GSYM length_flatten_eq_size_of_shape] >> fs []
+  rw []
+  \\ dep_rewrite.DEP_REWRITE_TAC [el_el_with_shape]
+  \\ simp []
+  \\ dep_rewrite.DEP_REWRITE_TAC [update_eq_zip_flookup]
+  \\ qspecl_then [`args`, `n`] assume_tac LESS_LENGTH
+  \\ qspecl_then [`sh`, `n`] assume_tac LESS_LENGTH
+  \\ gs [EL_APPEND1, EL_APPEND2, TAKE_APPEND1, TAKE_LENGTH_TOO_LONG]
+  \\ gs [listTheory.LIST_REL_APPEND_EQ, length_flatten_eq_size_of_shape]
+  \\ imp_res_tac list_rel_length_shape_of_flatten_better
+  \\ simp [EL_APPEND1, EL_APPEND2, length_flatten_eq_size_of_shape]
 QED
+
+Theorem opt_mmap_helper_thm[local] =
+  Q.SPECL [`es`, `es`] OPT_MMAP_CONG
+    |> Q.ISPEC `\e. eval ((if T then f else I) st) e`
+    |> Q.SPEC `\e. eval st e`
+    |> REWRITE_RULE []
+    |> Q.GENL [`f`, `st`, `es`]
 
 Theorem eval_upd_clock_eq:
   !t e ck. eval (t with clock := ck) e =  eval t e
 Proof
   ho_match_mp_tac eval_ind >> rw [] >>
   fs [eval_def] >>
-  qsuff_tac ‘OPT_MMAP (λa. eval (t with clock := ck) a) es =
-             OPT_MMAP (λa. eval t a) es’ >>
-  fs [] >>
-  pop_assum mp_tac >>
-   qid_spec_tac ‘es’ >>
-   Induct >> rw [] >>
-   fs [OPT_MMAP_def]
+  gs [Q.SPEC `clock_fupd g` opt_mmap_helper_thm] >>
+  rpt ((pairarg_tac ORELSE TOP_CASE_TAC) >> fs []) >>
+  gs [Q.SPEC `clock_fupd g` opt_mmap_helper_thm]
 QED
 
 Theorem eval_upd_code_eq:
@@ -498,13 +487,9 @@ Theorem eval_upd_code_eq:
 Proof
   ho_match_mp_tac eval_ind >> rw [] >>
   fs [eval_def] >>
-  qsuff_tac ‘OPT_MMAP (λa. eval (t with code := code) a) es =
-             OPT_MMAP (λa. eval t a) es’ >>
-  fs [] >>
-  pop_assum mp_tac >>
-  qid_spec_tac ‘es’ >>
-  Induct >> rw [] >>
-  fs [OPT_MMAP_def]
+  gs [Q.SPEC `code_fupd g` opt_mmap_helper_thm] >>
+  rpt ((pairarg_tac ORELSE TOP_CASE_TAC) >> fs []) >>
+  gs [Q.SPEC `code_fupd g` opt_mmap_helper_thm]
 QED
 
 Theorem opt_mmap_eval_upd_clock_eq:
@@ -605,8 +590,8 @@ Proof
       rpt(pairarg_tac >> gvs[]) >>
       gvs[AllCaseEqs(),dec_clock_def] >>
       imp_res_tac evaluate_clock >>
-      gvs[]
-      >- rw[state_component_equality] >>
+      gvs[] >>
+      simp [REWRITE_RULE [EQ_IMP_THM] state_component_equality] >>
       last_x_assum $ qspecl_then [‘st'' with clock := st''.clock - ck’,‘ck’] mp_tac >>
       (impl_tac >- gvs[state_component_equality]) >>
       strip_tac >>
@@ -868,46 +853,38 @@ Proof
   gvs[empty_locals_def,dec_clock_def]
 QED
 
+Theorem not_mem_map_flat[local]:
+  ~ MEM y (FLAT (MAP f xs)) = (!x. MEM x xs ==> ~ MEM y (f x))
+Proof
+  simp [MEM_MAP, MEM_FLAT]
+  \\ metis_tac []
+QED
+
+Theorem update_locals_not_vars_eval_eq_eq:
+  ∀s e v n w.
+  ~MEM n (var_exp e) ==>
+  eval (s with locals := s.locals |+ (n,w)) e = eval s e
+Proof
+  ho_match_mp_tac eval_ind >>
+  rpt conj_tac >> rpt gen_tac >>
+  simp [var_exp_def, eval_def, FLOOKUP_UPDATE, bool_case_eq] >>
+  rpt ((TOP_CASE_TAC ORELSE pairarg_tac) \\ fs []) >>
+  csimp [Q.SPEC `locals_fupd foo` opt_mmap_helper_thm] >>
+  rw [] >>
+  full_simp_tac bool_ss [o_DEF, EXISTS_NOT_EVERY] >>
+  gvs [UNZIP_MAP, MEM_MAP, FORALL_PROD, PULL_EXISTS] >>
+  gs [not_mem_map_flat, MEM_MAP, FORALL_PROD, PULL_EXISTS,
+        SF SFY_ss, Q.SPEC `locals_fupd foo` opt_mmap_helper_thm] >>
+  full_simp_tac bool_ss [o_DEF, EXISTS_NOT_EVERY, SF SFY_ss]
+QED
+
 Theorem update_locals_not_vars_eval_eq:
   ∀s e v n w.
   ~MEM n (var_exp e) /\
   eval s e = SOME v ==>
   eval (s with locals := s.locals |+ (n,w)) e = SOME v
 Proof
-  ho_match_mp_tac eval_ind >>
-  rpt conj_tac >> rpt gen_tac
-  >~ [‘Struct’]
-  >- (fs [var_exp_def] >>
-      rpt strip_tac >>
-      gvs[eval_def,AllCaseEqs()] >>
-      imp_res_tac opt_mmap_el >>
-      imp_res_tac opt_mmap_length_eq >>
-      gvs[opt_mmap_eq_some] >>
-      irule LIST_EQ >>
-      rw[EL_MAP] >>
-      first_x_assum irule >>
-      simp[MEM_EL,PULL_EXISTS] >>
-      irule_at (Pos last) EQ_REFL >>
-      simp[] >>
-      rw[] >>
-      gvs[MEM_FLAT,MEM_MAP,MEM_EL,PULL_FORALL, SF DNF_ss] >>
-      metis_tac[]) >>
-  rw[] >>
-  gvs[eval_def,var_exp_def, lookup_kvar_def, FLOOKUP_UPDATE,AllCaseEqs(),
-      PULL_EXISTS] >>
-  ntac 2 $ first_assum $ irule_at $ Pos last >>
-  imp_res_tac opt_mmap_el >>
-  imp_res_tac opt_mmap_length_eq >>
-  gvs[opt_mmap_eq_some] >>
-  irule LIST_EQ >>
-  rw[EL_MAP] >>
-  first_x_assum irule >>
-  simp[MEM_EL,PULL_EXISTS] >>
-  irule_at (Pos last) EQ_REFL >>
-  simp[] >>
-  rw[] >>
-  gvs[MEM_FLAT,MEM_MAP,MEM_EL,PULL_FORALL, SF DNF_ss] >>
-  metis_tac[]
+  simp [update_locals_not_vars_eval_eq_eq]
 QED
 
 Theorem update_locals_not_vars_eval_eq_NONE:
@@ -916,32 +893,7 @@ Theorem update_locals_not_vars_eval_eq_NONE:
   eval s e = NONE ==>
   eval (s with locals := s.locals |+ (n,w)) e = NONE
 Proof
-  ho_match_mp_tac eval_ind >>
-  rpt conj_tac >> rpt gen_tac
-  >~ [‘Struct’]
-  >- (fs [var_exp_def] >>
-      rpt strip_tac >>
-      gvs[eval_def,AllCaseEqs()] >>
-      ‘OPT_MMAP (λa. eval s a) es = OPT_MMAP (λa. eval (s with locals := s.locals |+ (n,w)) a) es’
-        by(qpat_x_assum ‘OPT_MMAP _ _ = _’ kall_tac >>
-           irule OPT_MMAP_CONG >>
-           rw[] >>
-           gvs[MEM_FLAT,MEM_MAP,SF DNF_ss] >>
-           Cases_on ‘eval s x’ >> gvs[] >>
-           metis_tac[update_locals_not_vars_eval_eq]) >>
-      gvs[]) >>
-  rw[] >>
-  gvs[eval_def,var_exp_def, lookup_kvar_def, FLOOKUP_UPDATE,AllCaseEqs(),PULL_EXISTS] >>
-  imp_res_tac update_locals_not_vars_eval_eq >>
-  gvs[] >>
-  ‘OPT_MMAP (λa. eval s a) es = OPT_MMAP (λa. eval (s with locals := s.locals |+ (n,w)) a) es’
-    by(qpat_x_assum ‘OPT_MMAP _ _ = _’ kall_tac >>
-       irule OPT_MMAP_CONG >>
-       rw[] >>
-       gvs[MEM_FLAT,MEM_MAP,SF DNF_ss] >>
-       Cases_on ‘eval s x’ >> gvs[] >>
-       metis_tac[update_locals_not_vars_eval_eq]) >>
-  gvs[]
+  simp [update_locals_not_vars_eval_eq_eq]
 QED
 
 Theorem eval_fresh_var:
@@ -1076,8 +1028,11 @@ QED
 Definition every_exp_def:
   (every_exp P (panLang$Const w) = P(Const w)) ∧
   (every_exp P (Var vk v) = P(Var vk v)) ∧
-  (every_exp P (Struct es) = (P(Struct es) ∧ EVERY (every_exp P) es)) ∧
-  (every_exp P (Field i e) = (P(Field i e) ∧ every_exp P e)) ∧
+  (every_exp P (RStruct es) = (P(RStruct es) ∧ EVERY (every_exp P) es)) ∧
+  (every_exp P (RField i e) = (P(RField i e) ∧ every_exp P e)) ∧
+  (every_exp P (NStruct nm nm_es) = (P(NStruct nm nm_es) ∧
+    EVERY (every_exp P) (MAP SND nm_es))) ∧
+  (every_exp P (NField i e) = (P(NField i e) ∧ every_exp P e)) ∧
   (every_exp P (Load sh e) = (P(Load sh e) ∧ every_exp P e)) ∧
   (every_exp P (Load32 e) = (P(Load32 e) ∧ every_exp P e)) ∧
   (every_exp P (LoadByte e) = (P(LoadByte e) ∧ every_exp P e)) ∧
@@ -1090,10 +1045,9 @@ Definition every_exp_def:
   (every_exp P BytesInWord = P BytesInWord)
 Termination
   wf_rel_tac `measure (exp_size ARB o SND)` >>
-  rpt strip_tac >>
-  imp_res_tac MEM_IMP_exp_size >>
-  TRY (first_x_assum (assume_tac o Q.SPEC `ARB`)) >>
-  decide_tac
+  rw [] >>
+  fs [MEM_MAP, EXISTS_PROD] >>
+  fs [MEM_SPLIT, list_size_append]
 End
 
 Definition exps_of_def:
@@ -1125,8 +1079,10 @@ Definition localised_exp_def:
   (localised_exp (BytesInWord) = T) ∧
   (localised_exp (Var Local v) = T) ∧
   (localised_exp (Var Global v) = F) ∧
-  (localised_exp (Struct es) = EVERY localised_exp es) ∧
-  (localised_exp (Field i e) = localised_exp e) ∧
+  (localised_exp (RStruct es) = EVERY localised_exp es) ∧
+  (localised_exp (RField i e) = localised_exp e) ∧
+  (localised_exp (NStruct nm nm_es) = EVERY localised_exp (MAP SND nm_es)) ∧
+  (localised_exp (NField i e) = localised_exp e) ∧
   (localised_exp (Load sh e) = localised_exp e) ∧
   (localised_exp (Load32 e) = localised_exp e) ∧
   (localised_exp (LoadByte e) = localised_exp e) ∧
@@ -1135,12 +1091,20 @@ Definition localised_exp_def:
   (localised_exp (Cmp c e1 e2) = (localised_exp e1 ∧ localised_exp e2)) ∧
   (localised_exp (Shift sh e num) = localised_exp e)
 Termination
-  wf_rel_tac `measure (\e. exp_size ARB e)` >>
-  rpt strip_tac >>
-  imp_res_tac MEM_IMP_exp_size >>
-  TRY (first_x_assum (assume_tac o Q.SPEC `ARB`)) >>
-  decide_tac
+  wf_rel_tac `measure (exp_size ARB)` >>
+  rw [] >>
+  fs [MEM_MAP, EXISTS_PROD] >>
+  fs [MEM_SPLIT, list_size_append]
 End
+
+(* Sigh. *)
+Theorem localised_exp_eq_every_exp:
+  !e. localised_exp e = every_exp (\e. case e of Var Global _ => F | _ => T) e
+Proof
+  recInduct localised_exp_ind
+  \\ simp [localised_exp_def, every_exp_def]
+  \\ rw [EVERY_CONG]
+QED
 
 Definition localised_prog_def:
   (localised_prog (Raise _ e) ⇔ localised_exp e) ∧
@@ -1174,10 +1138,15 @@ Theorem evaluate_decl_commute:
   evaluate_decls s (Function fi::Decl sh v' e::ds) =
   evaluate_decls s (Decl sh v' e::Function fi::ds)
 Proof
-  rw[evaluate_decls_def] >>
-  irule option_case_cong >> simp[] >>
-  PURE_REWRITE_TAC[Once $ GSYM state_fupdcanon] >>
-  irule eval_upd_code_eq
+  rw[evaluate_decls_def]
+  >- (
+    irule option_case_cong >> simp[] >>
+    PURE_REWRITE_TAC[Once $ GSYM state_fupdcanon] >>
+    irule eval_upd_code_eq
+  )
+  >- (
+    TOP_CASE_TAC >> simp []
+  )
 QED
 
 Theorem functions_eq_FILTER:
@@ -1225,17 +1194,6 @@ Proof
   simp[state_component_equality]
 QED
 
-Theorem evaluate_decls_only_functions':
-  ∀s pan_code.
-    EVERY is_function pan_code ⇒
-    evaluate_decls s pan_code = SOME(s with code := s.code |++ functions pan_code)
-Proof
-  recInduct evaluate_decls_ind >>
-  rw[evaluate_decls_def,functions_def,FUPDATE_LIST_THM] >>
-  gvs[AllCaseEqs(),is_function_def] >>
-  simp[state_component_equality]
-QED
-
 Theorem evaluate_decls_append:
   ∀s ds1 ds2.
     evaluate_decls s (ds1 ++ ds2) =
@@ -1248,21 +1206,25 @@ Proof
   ntac 2 (TOP_CASE_TAC >> gvs[])
 QED
 
+Theorem opt_mmap_eq_some_helper[local]:
+  !xs zs. OPT_MMAP f xs = SOME zs /\
+  (!x. MEM x xs ==> !y. f x = SOME y ==> g x = SOME y) ==>
+  OPT_MMAP g xs = SOME zs
+Proof
+  Induct_on `xs`
+  \\ rw []
+QED
+
 Theorem eval_empty_locals_IMP:
   ∀s e v.
     eval (s with locals := FEMPTY) e = SOME v ⇒
     eval s e = SOME v
 Proof
   recInduct eval_ind >>
-  rw[eval_def,AllCaseEqs(),PULL_EXISTS] >>
+  rw[eval_def,AllCaseEqs(),PULL_EXISTS,UNZIP_MAP] >>
   res_tac >> gvs[] >>
-  rpt $ first_assum $ irule_at(Pos last) >>
-  irule EQ_TRANS >>
-  first_assum $ irule_at $ Pos last >>
-  irule OPT_MMAP_CONG >>
-  rw[] >>
-  drule_all pan_commonPropsTheory.opt_mmap_mem_func >>
-  strip_tac >> gvs[]
+  dxrule_then (irule_at Any) opt_mmap_eq_some_helper >>
+  simp []
 QED
 
 Theorem semantics_decls_has_main:
@@ -1311,43 +1273,50 @@ Proof
 QED
 
 Theorem mem_load_swap_memory:
-  (∀sh (addr:'a word) addrs memory1 v memory2.
-    mem_load sh addr addrs memory1 = SOME v ∧
+  (∀sh (addr:'a word) addrs memory1 stcs v memory2.
+    mem_load sh addr addrs memory1 stcs = SOME v ∧
     (∀addr. addr ∈ addrs ⇒ memory1 addr = memory2 addr)
     ⇒
-    mem_load sh addr addrs memory2 = SOME v) ∧
-  (∀shs (addr:'a word) addrs memory1 v memory2.
-    mem_loads shs addr addrs memory1 = SOME v ∧
+    mem_load sh addr addrs memory2 stcs = SOME v) ∧
+  (∀shs (addr:'a word) addrs memory1 stcs v memory2.
+    mem_loads shs addr addrs memory1 stcs = SOME v ∧
     (∀addr. addr ∈ addrs ⇒ memory1 addr = memory2 addr)
     ⇒
-    mem_loads shs addr addrs memory2 = SOME v)
+    mem_loads shs addr addrs memory2 stcs = SOME v) ∧
+  (∀flds (addr:'a word) addrs memory1 stcs vs memory2.
+   mem_load_flds flds addr addrs memory1 stcs = SOME vs ∧
+    (∀addr. addr ∈ addrs ⇒ memory1 addr = memory2 addr)
+    ⇒
+    mem_load_flds flds addr addrs memory2 stcs = SOME vs)
 Proof
-  Induct >>
-  simp[cj 1 mem_load_def] >>
-  simp[cj 2 mem_load_def, cj 3 mem_load_def] >>
-  rw[AllCaseEqs()] >>
-  res_tac >>
-  fs[]
+  ho_match_mp_tac mem_load_ind >>
+  rw [mem_load_def] >>
+  fs [AllCaseEqs()] >>
+  gvs []
 QED
 
 Theorem mem_load_swap_memaddrs:
-  (∀sh (addr:'a word) addrs memory v addrs2.
-    mem_load sh addr addrs memory = SOME v ∧
+  (∀sh (addr:'a word) addrs memory stcs v addrs2.
+    mem_load sh addr addrs memory stcs = SOME v ∧
     addrs ⊆ addrs2
     ⇒
-    mem_load sh addr addrs2 memory = SOME v) ∧
-  (∀shs (addr:'a word) addrs memory v addrs2.
-    mem_loads shs addr addrs memory = SOME v ∧
+    mem_load sh addr addrs2 memory stcs = SOME v) ∧
+  (∀shs (addr:'a word) addrs memory stcs v addrs2.
+    mem_loads shs addr addrs memory stcs = SOME v ∧
     addrs ⊆ addrs2
     ⇒
-    mem_loads shs addr addrs2 memory = SOME v)
+    mem_loads shs addr addrs2 memory stcs = SOME v) ∧
+  (∀flds (addr:'a word) addrs memory stcs vs addrs2.
+   mem_load_flds flds addr addrs memory stcs = SOME vs ∧
+    addrs ⊆ addrs2
+    ⇒
+    mem_load_flds flds addr addrs2 memory stcs = SOME vs)
 Proof
-  Induct >>
-  simp[cj 1 mem_load_def] >>
-  simp[cj 2 mem_load_def, cj 3 mem_load_def] >>
-  rw[AllCaseEqs()] >>
-  res_tac >>
-  fs[SUBSET_DEF]
+  ho_match_mp_tac mem_load_ind >>
+  rw [mem_load_def] >>
+  fs [AllCaseEqs()] >>
+  gvs [] >>
+  imp_res_tac SUBSET_IMP
 QED
 
 Theorem eval_swap_memaddrs:
@@ -1358,19 +1327,11 @@ Theorem eval_swap_memaddrs:
     eval (s with memaddrs := memaddrs) exp = SOME v
 Proof
   recInduct eval_ind >>
-  rw[eval_def,AllCaseEqs(),PULL_EXISTS,mem_load_byte_def,mem_load_32_alt] >>
-  rpt $ irule_at (Pos last) EQ_REFL >>
-  rpt $ first_assum $ irule_at (Pos last) >>
-  fs[]
-  >~ [‘mem_load’]
-  >- (irule $ cj 1 mem_load_swap_memaddrs >> metis_tac[]) >>
-  fs[SUBSET_DEF] >>
-  irule EQ_TRANS >>
-  first_assum $ irule_at $ Pos last >>
-  irule OPT_MMAP_CONG >>
-  rw[] >>
-  drule_all_then strip_assume_tac pan_commonPropsTheory.opt_mmap_mem_func >>
-  gvs[]
+  rw[eval_def,AllCaseEqs(),PULL_EXISTS,UNZIP_MAP,mem_load_byte_def,mem_load_32_alt] >>
+  res_tac >> simp [] >>
+  imp_res_tac SUBSET_IMP >>
+  imp_res_tac mem_load_swap_memaddrs >>
+  dxrule_then (irule_at Any) opt_mmap_eq_some_helper >> simp []
 QED
 
 Theorem evaluate_decls_swap_memaddrs:
@@ -1397,18 +1358,12 @@ Theorem eval_swap_memory:
     eval (s with memory := mry) exp = SOME v
 Proof
   recInduct eval_ind >>
-  rw[eval_def,AllCaseEqs(),PULL_EXISTS,mem_load_byte_def,mem_load_32_alt] >>
-  rpt $ irule_at (Pos last) EQ_REFL >>
-  rpt $ first_assum $ irule_at (Pos last) >>
-  fs[]
-  >~ [‘mem_load’]
-  >- (irule $ cj 1 mem_load_swap_memory >> metis_tac[]) >>
-  irule EQ_TRANS >>
-  first_assum $ irule_at $ Pos last >>
-  irule OPT_MMAP_CONG >>
-  rw[] >>
-  drule_all_then strip_assume_tac pan_commonPropsTheory.opt_mmap_mem_func >>
-  gvs[]
+  rw[eval_def,AllCaseEqs(),PULL_EXISTS,UNZIP_MAP,mem_load_byte_def,mem_load_32_alt] >>
+  res_tac >> simp [] >>
+  imp_res_tac SUBSET_IMP >>
+  imp_res_tac mem_load_swap_memory >>
+  fs [] >>
+  dxrule_then (irule_at Any) opt_mmap_eq_some_helper >> simp []
 QED
 
 Theorem evaluate_decls_swap_memory:
